contents -> descriptor

ulib/experimental/Steel.PCM.ArrayStruct.Memory.fst
@@ -22,40 +22,39 @@ open Steel.PCM
 type usize = U32.t
 let v_usize = U32.v
 
-//TODO: change contents to descriptor
 //TODO: use Steel.SizeT
 
 #set-options "--fuel 1 --ifuel 1"
 
-noeq type array_struct_contents : Type u#(a+1) =
-  | Base: a: Type u#a -> pcm: pcm a -> array_struct_contents
-  | Array: t:array_struct_contents u#a -> len:usize -> array_struct_contents
+noeq type array_struct_descriptor : Type u#(a+1) =
+  | Base: a: Type u#a -> pcm: pcm a -> array_struct_descriptor
+  | Array: t:array_struct_descriptor u#a -> len:usize -> array_struct_descriptor
 
-let rec array_struct_type (contents: array_struct_contents) : Tot Type (decreases contents) =
-  match contents with
+let rec array_struct_type (descriptor: array_struct_descriptor) : Tot Type (decreases descriptor) =
+  match descriptor with
   | Base a pcm -> a
-  | Array contents' len ->
-    let type' = array_struct_type contents' in
+  | Array descriptor' len ->
+    let type' = array_struct_type descriptor' in
     Seq.lseq type' (v_usize len)
 
 noeq type array_struct : Type u#(a+1) =
   | ArrayStruct:
-    contents: array_struct_contents u#a ->
-    value:(array_struct_type contents) ->
+    descriptor: array_struct_descriptor u#a ->
+    value:(array_struct_type descriptor) ->
     array_struct
 
-let rec composable_array_struct' (s0 s1: array_struct) : Tot prop (decreases s0.contents) =
-  match s0.contents, s1.contents with
+let rec composable_array_struct' (s0 s1: array_struct) : Tot prop (decreases s0.descriptor) =
+  match s0.descriptor, s1.descriptor with
   | Base a0 pcm0, Base a1 pcm1 ->
     a0 == a1 /\ pcm0 == pcm1 /\
     composable pcm0 s0.value s1.value
-  | Array contents0 len0, Array contents1 len1 ->
-    contents0 == contents1 /\ len0 == len1 /\
+  | Array descriptor0 len0, Array descriptor1 len1 ->
+    descriptor0 == descriptor1 /\ len0 == len1 /\
     begin forall (i:nat{i < v_usize len0}).
       let val0 = Seq.index s0.value i in
       let val1 = Seq.index s1.value i in
-      let sub_s0 = ArrayStruct contents0 val0 in
-      let sub_s1 = ArrayStruct contents1 val1 in
+      let sub_s0 = ArrayStruct descriptor0 val0 in
+      let sub_s1 = ArrayStruct descriptor1 val1 in
       composable_array_struct' sub_s0 sub_s1
     end
   | _ -> False
@@ -64,25 +63,25 @@ let rec composable_sym (s0 s1: array_struct)
     : Lemma
       (requires True)
       (ensures (composable_array_struct' s0 s1 <==> composable_array_struct' s1 s0))
-      (decreases s0.contents)
+      (decreases s0.descriptor)
   =
-  match s0.contents, s1.contents with
+  match s0.descriptor, s1.descriptor with
   | Base a0 pcm0, Base a1 pcm1 ->
     ()
-  | Array contents0 len0, Array contents1 len1 ->
+  | Array descriptor0 len0, Array descriptor1 len1 ->
     let aux (_ : squash (composable_array_struct' s0 s1))
         : Lemma (composable_array_struct' s1 s0) =
       let aux (i:nat{i < v_usize len0}) : Lemma (
         let val0 = Seq.index s0.value i in
         let val1 = Seq.index s1.value i in
-        let sub_s0 = ArrayStruct contents0 val0 in
-        let sub_s1 = ArrayStruct contents1 val1 in
+        let sub_s0 = ArrayStruct descriptor0 val0 in
+        let sub_s1 = ArrayStruct descriptor1 val1 in
         composable_array_struct' sub_s1 sub_s0
       ) =
         let val0 = Seq.index s0.value i in
         let val1 = Seq.index s1.value i in
-        let sub_s0 = ArrayStruct contents0 val0 in
-        let sub_s1 = ArrayStruct contents1 val1 in
+        let sub_s0 = ArrayStruct descriptor0 val0 in
+        let sub_s1 = ArrayStruct descriptor1 val1 in
         composable_sym sub_s0 sub_s1
       in
       Classical.forall_intro aux
@@ -93,14 +92,14 @@ let rec composable_sym (s0 s1: array_struct)
       let aux (i:nat{i < v_usize len0}) : Lemma (
         let val0 = Seq.index s0.value i in
         let val1 = Seq.index s1.value i in
-        let sub_s0 = ArrayStruct contents0 val0 in
-        let sub_s1 = ArrayStruct contents1 val1 in
+        let sub_s0 = ArrayStruct descriptor0 val0 in
+        let sub_s1 = ArrayStruct descriptor1 val1 in
         composable_array_struct' sub_s0 sub_s1
       ) =
         let val0 = Seq.index s0.value i in
         let val1 = Seq.index s1.value i in
-        let sub_s0 = ArrayStruct contents0 val0 in
-        let sub_s1 = ArrayStruct contents1 val1 in
+        let sub_s0 = ArrayStruct descriptor0 val0 in
+        let sub_s1 = ArrayStruct descriptor1 val1 in
         composable_sym sub_s0 sub_s1
       in
       Classical.forall_intro aux
@@ -115,25 +114,25 @@ let composable_array_struct : symrel array_struct =
 let rec compose_array_struct
   (s0 : array_struct)
   (s1: array_struct{s0 `composable_array_struct` s1})
-    : Tot (s':array_struct{s'.contents == s0.contents})
-      (decreases s0.contents)
+    : Tot (s':array_struct{s'.descriptor == s0.descriptor})
+      (decreases s0.descriptor)
   =
-  match s0.contents, s1.contents with
+  match s0.descriptor, s1.descriptor with
   | Base a0 pcm0, Base a1 pcm1 ->
-    ArrayStruct s0.contents (op pcm0 s0.value s1.value)
-  | Array contents0 len0, Array contents1 len1 ->
-    let new_val : Seq.lseq (array_struct_type contents0) (v_usize len0) =
+    ArrayStruct s0.descriptor (op pcm0 s0.value s1.value)
+  | Array descriptor0 len0, Array descriptor1 len1 ->
+    let new_val : Seq.lseq (array_struct_type descriptor0) (v_usize len0) =
       Seq.init (v_usize len0) (fun i ->
         let val0 = Seq.index s0.value i in
         let val1 = Seq.index s1.value i in
-        let sub_s0 = ArrayStruct contents0 val0 in
-        let sub_s1 = ArrayStruct contents1 val1 in
+        let sub_s0 = ArrayStruct descriptor0 val0 in
+        let sub_s1 = ArrayStruct descriptor1 val1 in
         let new_as : array_struct = compose_array_struct sub_s0 sub_s1 in
-        let out : (array_struct_type contents0) = new_as.value in
+        let out : (array_struct_type descriptor0) = new_as.value in
         out
       )
     in
-    ArrayStruct s0.contents new_val
+    ArrayStruct s0.descriptor new_val
 
 let one_pcm : pcm unit = {
   p = {
